theories/zoo/language/state.v
@@ -1,0 +1,133 @@
+From stdpp Require Import
+  gmap.
+
+From iris.algebra Require Import
+  ofe.
+
+From zoo Require Import
+  prelude.
+From zoo.language Require Export
+  syntax.
+From zoo Require Import
+  options.
+
+Implicit Types l : location.
+Implicit Types v w : val.
+Implicit Types vs : list val.
+
+Record header := Header {
+  header_tag : nat ;
+  header_size : nat ;
+}.
+Add Printing Constructor header.
+
+Record state := {
+  state_headers : gmap location header ;
+  state_heap : gmap location val ;
+  state_locals : list val ;
+  state_prophets : gset prophet_id ;
+}.
+Implicit Types σ : state.
+
+Canonical state_O {SI : sidx} :=
+  leibnizO state.
+
+#[global] Instance state_inhabited : Inhabited state :=
+  populate
+    {|state_headers := inhabitant ;
+      state_heap := inhabitant ;
+      state_locals := inhabitant ;
+      state_prophets := inhabitant ;
+    |}.
+
+Definition state_update_heap f σ :=
+  {|state_headers := σ.(state_headers) ;
+    state_heap := f σ.(state_heap) ;
+    state_locals := σ.(state_locals) ;
+    state_prophets := σ.(state_prophets) ;
+  |}.
+Definition state_update_headers f σ :=
+  {|state_headers := f σ.(state_headers) ;
+    state_heap := σ.(state_heap) ;
+    state_locals := σ.(state_locals) ;
+    state_prophets := σ.(state_prophets) ;
+  |}.
+Definition state_update_locals f σ :=
+  {|state_headers := σ.(state_headers) ;
+    state_heap := σ.(state_heap) ;
+    state_locals := f σ.(state_locals) ;
+    state_prophets := σ.(state_prophets) ;
+  |}.
+Definition state_update_prophets f σ :=
+  {|state_headers := σ.(state_headers) ;
+    state_heap := σ.(state_heap) ;
+    state_locals := σ.(state_locals) ;
+    state_prophets := f σ.(state_prophets) ;
+  |}.
+
+Definition state_set_location l v :=
+  state_update_heap $ insert l v.
+Definition state_set_header l hdr :=
+  state_update_headers $ insert l hdr.
+Definition state_set_local tid v :=
+  state_update_locals $ insert tid v.
+Definition state_add_local v :=
+  state_update_locals $ (.++ [v]).
+Definition state_add_prophet pid :=
+  state_update_prophets $ ({[pid]} ∪.).
+
+Fixpoint heap_array l vs : gmap location val :=
+  match vs with
+  | [] =>
+      ∅
+  | v :: vs =>
+      <[l := v]> (heap_array (l +ₗ 1) vs)
+  end.
+#[global] Arguments heap_array _ !_ / : assert.
+
+Lemma heap_array_singleton l v :
+  heap_array l [v] = {[l := v]}.
+Proof.
+  rewrite /heap_array insert_empty //.
+Qed.
+Lemma heap_array_lookup l vs w k :
+  heap_array l vs !! k = Some w ↔
+    ∃ j,
+    (0 ≤ j)%Z ∧
+    k = l +ₗ j ∧
+    vs !! ₊j = Some w.
+Proof.
+  revert k l; induction vs as [|v' vs IH]=> l' l /=.
+  { rewrite lookup_empty. naive_solver lia. }
+  rewrite lookup_insert_Some IH. split.
+  - intros [[-> ?] | (Hl & j & ? & -> & ?)].
+    { eexists 0. rewrite location_add_0. naive_solver lia. }
+    eexists (1 + j)%Z. rewrite location_add_assoc !Z.add_1_l Z2Nat.inj_succ; auto with lia.
+  - intros (j & ? & -> & Hil). destruct_decide (j = 0); simplify_eq/=.
+    { rewrite location_add_0; eauto. }
+    right. split.
+    { rewrite -{1}(location_add_0 l). intros ?%(inj (location_add _)); lia. }
+    assert (₊j = S ₊(j - 1)) as Hj.
+    { rewrite -Z2Nat.inj_succ; last lia. f_equal; lia. }
+    rewrite Hj /= in Hil.
+    eexists (j - 1)%Z. rewrite location_add_assoc Z.add_sub_assoc Z.add_simpl_l. auto with lia.
+Qed.
+Lemma heap_array_map_disjoint heap l vs :
+  ( ∀ i,
+    i < length vs →
+    heap !! (l +ₗ i) = None
+  ) →
+  heap_array l vs ##ₘ heap.
+Proof.
+  intros Hdisj. apply map_disjoint_spec=> l' v1 v2.
+  intros (j & ? & -> & ?%lookup_lt_Some%inj_lt)%heap_array_lookup ?.
+  ospecialize* (Hdisj ₊j); first lia.
+  rewrite Z2Nat.id // in Hdisj. naive_solver.
+Qed.
+
+Definition state_alloc l hdr vs σ :=
+  {|state_headers := <[l := hdr]> σ.(state_headers) ;
+    state_heap := heap_array l vs ∪ σ.(state_heap) ;
+    state_locals := σ.(state_locals) ;
+    state_prophets := σ.(state_prophets) ;
+  |}.
